wrote some contracty stuff BlockCache

disk-betree/BlockCache.dfy
@@ -4,22 +4,40 @@ abstract module BlockCache {
 
   type Reference(!new,==)
 
-  function View<T>(k: Constants, s: Variables) : imap<Reference, T>
-    ensures forall ref :: ref in View(k, s)
+  type View<T> = imap<Reference, T>
+    
+  function ViewOf<T>(k: Constants, s: Variables) : View
     
   function Read<T>(k: Constants, s: Variables, ref: Reference) : T
-    ensures Read(k, s, ref) == View(k, s)[ref];
+    requires ref in ViewOf(k, s)
+    ensures Read(k, s, ref) == ViewOf(k, s)[ref];
     
   datatype CacheOp<T> =
     | AllocOp(block: T, successors: iset<Reference>, new_ref: Reference)
     | WriteOp(ref: Reference, block: T, successors: iset<Reference>)
     
-  predicate Apply(k: Constants, s: Variables, s': Variables, op: CacheOp)
+  function ApplyToView(view: View, op: CacheOp) : View {
+    match op {
+      case AllocOp(block, successors, new_ref) => view[op.new_ref := op.block]
+      case WriteOp(ref, block, successors) => view[op.ref := op.block]
+    }
+  }
     
-  predicate Apply2(k: Constants, s: Variables, s': Variables, op1: CacheOp, op2: CacheOp) {
+  predicate Apply(k: Constants, s: Variables, s': Variables, op: CacheOp)
+    requires op.AllocOp? ==> op.new_ref !in ViewOf(k, s)
+    ensures Apply(k, s, s', op) ==> ViewOf(k, s') == ApplyToView(ViewOf(k, s), op)
+    
+  predicate Apply2(k: Constants, s: Variables, s': Variables, op1: CacheOp, op2: CacheOp)
+    requires op1.AllocOp? ==> op1.new_ref !in ViewOf(k, s)
+    requires op2.AllocOp? ==> op2.new_ref !in ApplyToView(ViewOf(k, s), op1)
+    ensures Apply2(k, s, s', op1, op2) ==> ViewOf(k, s') == ApplyToView(ApplyToView(ViewOf(k, s), op1), op2)
+  {
     exists sint :: 
       && Apply(k, s, sint, op1)
+      && assert ViewOf(k, sint) == ApplyToView(ViewOf(k, s), op1);
       && Apply(k, sint, s', op2)
+      && assert ViewOf(k, s') == ApplyToView(ViewOf(k, sint), op2);
+      && true
   }
     
   function Root(k: Constants) : Reference
